theories/Syntax/Resource.v
@@ -1,16 +1,24 @@
 From Coq Require Import Lia PeanoNat.
-From DeBrLevel Require Import LevelInterface Level PairLevel.
+From DeBrLevel Require Import LevelInterface Level Levels SetLevelInterface.
 
 (** * Syntax - Resource
 
-  A resource is a kind of reference defined in the Wormholes language. Like a variable,
-  we need identifiers for resources. Thus, we choose De Bruijn level as representation in
-  order to avoid capture variables. It is a direct use of the [Level] module.
+  Resources are names that are either bound to I/O or introduced by the binder wh as local references.
+  The original paper defines a resource as an element taken from an infinite countable set.
+  We choose De-Bruijn level as representation which avoid captures issues. Consequently, a resource is 
+  a level. It is a direct use of the [Level] module.
 *)
 Module Resource <: IsBdlLvlFullOTWL.
 
 Include Level.
 
+(** ** Multi shift 
+
+During the functional transition, defined in [FT_Definition], the signal function is updated multiple 
+times with different lower bound and shift value. Thus, we define a [multi_shift] function that applies
+[n] shifts for two lists [lbs] and [ks] of length [n].
+
+*)
 Definition multi_shift (lbs : list nat) (ks : list nat) (t : t) :=
   List.fold_right (fun (x : nat * nat) acc => let (lb,k) := x in shift lb k acc) t (List.combine lbs ks).
 
@@ -29,25 +37,90 @@ Proof.
     -- intros. apply H0; simpl; now right.
 Qed.
 
-
 End Resource.
 
-(** *** Scope and Notations *)
-Declare Custom Entry wormholes.
+(** * Syntax - Resources
+
+  Wormholes types contains a "reactive" arrow that carries a set of resources used
+  by the signal function. We define a set of resource directly via the [Levels] 
+  implementation contained in the library.
+*)
+Module Resources <: IsBdlLvlFullSetOTWLInterface Level.
+
+Include Levels.
+
+(** ** Multi shift 
+
+During the functional transition, defined in [FT_Definition], the signal function is updated multiple 
+times with different lower bound and shift value. Thus, we define a [multi_shift] function that applies
+[n] shifts for two lists [lbs] and [ks] of length [n].
+
+*)
+Definition multi_shift (lbs : list nat) (ks : list nat) (t : t) :=
+  List.fold_right (fun (x : nat * nat) acc => let (lb,k) := x in shift lb k acc) t (List.combine lbs ks).
+
+(** ** Wormholes specifcation *)
+
+Lemma valid_wh_spec : forall s lb,
+  valid (S (S lb)) s -> valid lb (diff s (add lb (add (S lb) empty))).
+Proof.
+  intros; rewrite valid_unfold in *; unfold For_all in *; 
+  intros. rewrite diff_spec in H0; destruct H0.
+  rewrite add_notin_spec in H1; destruct H1; 
+  rewrite add_notin_spec in H2; destruct H2; clear H3.
+  unfold Level.valid in *; apply H in H0; lia.
+Qed.
+
+End Resources.
+
+(** * Notation - Resource *)
+Module ResourceNotations.
+
+(** ** Scope *)
+Declare Custom Entry wh.
 Declare Scope resource_scope.
 Delimit Scope resource_scope with r.
-Definition resource := Resource.t.
+Declare Scope resources_scope.
+Delimit Scope resources_scope with rs.
 
-Notation "<[ e ]>" := e (e custom wormholes at level 99).
-Notation "( x )"   := x (in custom wormholes, x at level 99).
-Notation "x"       := x (in custom wormholes at level 0, x constr at level 0).
-Notation "{ x }"   := x (in custom wormholes at level 1, x constr).
+(** ** Notations *)
+Definition resource := Resource.t.
+Definition resources := Resources.t.
+
+Notation "<[ e ]>" := e (e custom wh at level 99).
+Notation "( x )"   := x (in custom wh, x at level 99).
+Notation "x"       := x (in custom wh at level 0, x constr at level 0).
+Notation "{ x }"   := x (in custom wh at level 1, x constr).
 
 Infix "<"  := Resource.lt : resource_scope.
-Infix "=" := Resource.eq : resource_scope.
-Infix "<?"  := Resource.ltb (at level 70) : resource_scope.
+Infix "="  := Resource.eq : resource_scope.
+Infix "<?" := Resource.ltb (at level 70) : resource_scope.
 Infix "=?" := Resource.eqb  (at level 70) : resource_scope.
 Infix "⊩ᵣ" := Resource.valid (at level 20, no associativity). 
 Infix "⊩?ᵣ" := Resource.validb (at level 20, no associativity). 
 Notation "'[⧐ᵣ' lb '≤' k ']' t" := (Resource.shift lb k t) (at level 65, right associativity).
 Notation "'[⧐⧐ᵣ' lb '≤' k ']' t" := (Resource.multi_shift lb k t) (at level 65, right associativity).
+
+Notation "∅ᵣₛ" := (Resources.empty).
+Notation "'\{{' x '}}'" := (Resources.singleton x).
+Notation "'\{{' x ';' y ';' .. ';' z '}}'" := (Resources.add x (Resources.add y .. (Resources.add z Resources.empty) .. )).
+Infix "∉"  := (fun x s => ~ Resources.In x s) (at level 75) : resources_scope.
+Infix "∈"  := (Resources.In)  (at level 60, no associativity) : resources_scope.
+Infix "+:" := (Resources.add)  (at level 60, no associativity) : resources_scope.
+Infix "∪"  := (Resources.union) (at level 50, left associativity) : resources_scope.
+Infix "∩"  := (Resources.inter) (at level 50, left associativity) : resources_scope.
+Infix "\"  := (Resources.diff) (at level 50, left associativity) : resources_scope.
+Infix "⊆"  := Resources.Subset (at level 60, no associativity) : resources_scope.
+Infix "⊈"  := (fun s s' => ~ (Resources.Subset s s')) (at level 60, no associativity) : resources_scope.
+
+Infix "<"  := Resources.lt : resources_scope.
+Infix "<?" := Resources.ltb (at level 70) : resources_scope.
+Infix "="  := Resources.eq : resources_scope.
+Infix "=?" := Resources.equal (at level 70) : resources_scope.
+
+Infix "⊩ᵣₛ" := Resources.valid (at level 20, no associativity). 
+Infix "⊩?ᵣₛ" := Resources.validb (at level 20, no associativity). 
+Notation "'[⧐ᵣₛ' lb '≤' k ']' t" := (Resources.shift lb k t) (at level 65, right associativity).
+Notation "'[⧐⧐ᵣₛ' lb '≤' k ']' t" := (Resources.multi_shift lb k t) (at level 65, right associativity).
+
+End ResourceNotations.
