theories/Transition/Evaluation/ET_Progress.v
@@ -1,7 +1,8 @@
 From Coq Require Import Lia.
-From Mecha Require Import Typ Resource Resources Term Var VContext RContext Typing ET_Definition.
+From Mecha Require Import Typ Resource Term Var VContext RContext Typing ET_Definition.
+Import ResourceNotations TypNotations TermNotations VContextNotations RContextNotations.
 
-(** * Progress *)
+(** * Transition - Evaluation - Progress *)
 
 (** ** Proof of progress of the evaluation transtion
 
@@ -13,19 +14,19 @@ From Mecha Require Import Typ Resource Resources Term Var VContext RContext Typi
 Theorem progress_of_evaluate : forall t Re τ,
                          ∅ᵥᵪ ⋅ Re ⊫ t ∈ τ -> 
 (*-----------------------------------------------------------------------*)
-     (* (1) *) value(t) \/ (* (2) *) exists t', (newᵣᵪ(Re)) ⊨ t ⟼ t'.
+     (* (1) *) value(t) \/ (* (2) *) exists t', Re⁺ᵣᵪ ⊨ t ⟼ t'.
 Proof.
   intro t; induction t; intros Re τ' Hwt; inversion Hwt; subst; 
   try (now left); try (apply IHt1 in H3 as H3'; apply IHt2 in H5 as H5').
   - destruct H3',H5'; right. 
-    -- inversion H; subst; inversion H3; subst. exists <[[x:= t2 ~ {newᵣᵪ(Re)} ≤ 0] t]>.
+    -- inversion H; subst; inversion H3; subst. exists <[[x:= t2 ~ {Re⁺ᵣᵪ} ≤ 0] t]>.
       now constructor.
     -- destruct H0; exists <[t1 x]>; now constructor.
     -- destruct H; exists <[x t2]>; now constructor.
     -- destruct H; exists <[x t2]>; now constructor.
   - right; apply IHt2 in H4 as H4'; destruct H4'.
     -- destruct t2; inversion H4; subst; inversion H; subst.
-        exists <[[v := Fix (\ v : τ', t2) ~ {newᵣᵪ(Re)} ≤ 0] t2]>; constructor.
+        exists <[[v := Fix (\ v : τ', t2) ~ {Re⁺ᵣᵪ} ≤ 0] t2]>; constructor.
     -- destruct H; exists <[Fix x]>; constructor; auto.
   - destruct H3',H5'; auto.
     -- right; destruct H0; exists <[⟨t1,x⟩]>; now constructor.
