theories/Transition/Functional/FT_Safety.v
@@ -3,6 +3,11 @@ From Coq Require Import Program Lia Relations.Relation_Definitions Classes.Relat
 From Mecha Require Import Resource Resources Term Typ Var ReadStock WriteStock Typing VContext RContext 
                           Cell REnvironment Stock ET_Definition ET_Props ET_Preservation 
                           FT_Definition FT_Props FT_Preservation FT_Progress.
+Import ResourceNotations TermNotations TypNotations CellNotations
+       VContextNotations RContextNotations REnvironmentNotations
+       ReadStockNotations WriteStockNotations StockNotations.
+       
+(** * Transition - Functional - Safety *)
 
 Section safety.
 
