theories/Transition/Temporal/TT_Definition.v
@@ -1,20 +1,20 @@
-From Mecha Require Import Resource Resources Term Typ Var ReadStock WriteStock Stock Typing
+From Mecha Require Import Resource Term Typ Var ReadStock WriteStock Stock Typing
                           Cell VContext REnvironment RContext ET_Definition FT_Definition
-                          RSample RSamples.
+                          Sample Samples.
+(**
 
 Definition temporal (S S1 : 𝐒) (P P' : Λ) (W W1 : 𝐖) :=
   forall Vin Vout Wnew _tv,
-    (Vin = Stock.init_virtual W (RSamples.nexts S))%re /\
+    (Vin = Stock.init_virtual W (Samples.nexts S))%re /\
                     
     ⪡ Vin ; unit ; P ⪢ ⭆ ⪡ Vout ; _tv ; P' ; Wnew ⪢ /\
                     
-    (S1 = RSamples.puts Vout S) /\ (W1 = Stock.update Wnew Vout)%sk. 
+    (S1 = Samples.puts Vout S) /\ (W1 = Stock.update Wnew Vout)%sk. 
 
 Notation "'⟦' S ';' W ';' P '⟧' '⟾' '⟦' S1 ';' W1 ';' P1 '⟧'" 
   := (temporal S S1 P P1 W W1) (at level 30, S constr, S1 constr,
-                                             P custom wormholes, P1 custom wormholes, 
+                                             P custom wh, P1 custom wh, 
                                              W constr, W1 constr, no associativity).
 
-(**
-The whole complete definition and proves will be available for the final version.
+
 *)
